\begin{align}
\begin{autobreak}
g_{G^{0} c_{W^{-}} \bar{c}_{W^{-}} }=
	-\frac{e \text{MW} \text{RXi}(W)}{2 s_W}
	,
\end{autobreak}
\end{align}
\begin{align}
\begin{autobreak}
g_{G^{0} c_{W^{+}} \bar{c}_{W^{+}} }=
	\frac{e \text{MW} \text{RXi}(W)}{2 s_W}
	,
\end{autobreak}
\end{align}
\begin{align}
\begin{autobreak}
g_{G^{-} c_{\gamma} \bar{c}_{W^{-}} }=
	i e \text{MW} \text{RXi}(W)
	,
\end{autobreak}
\end{align}
\begin{align}
\begin{autobreak}
g_{G^{-} c_{W^{+}} \bar{c}_{Z} }=
	\frac{i e \text{MZ} \text{RXi}(Z)}{2 s_W}
	,
\end{autobreak}
\end{align}
\begin{align}
\begin{autobreak}
g_{G^{-} c_{Z} \bar{c}_{W^{-}} }=
	-\frac{i e \text{MW} \text{RXi}(W)}{2 c_W s_W}
	+\frac{i e \text{MW} \text{RXi}(W) s_W}{c_W},
\end{autobreak}
\end{align}
\begin{align}
\begin{autobreak}
g_{G^{+} c_{\gamma} \bar{c}_{W^{+}} }=
	i e \text{MW} \text{RXi}(W)
	,
\end{autobreak}
\end{align}
\begin{align}
\begin{autobreak}
g_{G^{+} c_{W^{-}} \bar{c}_{Z} }=
	\frac{i e \text{MZ} \text{RXi}(Z)}{2 s_W}
	,
\end{autobreak}
\end{align}
\begin{align}
\begin{autobreak}
g_{G^{+} c_{Z} \bar{c}_{W^{+}} }=
	-\frac{i e \text{MW} \text{RXi}(W)}{2 c_W s_W}
	+\frac{i e \text{MW} \text{RXi}(W) s_W}{c_W},
\end{autobreak}
\end{align}
\begin{align}
\begin{autobreak}
g_{A c_{W^{-}} \bar{c}_{W^{-}} }=
	0
	,
\end{autobreak}
\end{align}
\begin{align}
\begin{autobreak}
g_{A c_{W^{+}} \bar{c}_{W^{+}} }=
	0
	,
\end{autobreak}
\end{align}
\begin{align}
\begin{autobreak}
g_{H c_{W^{-}} \bar{c}_{W^{-}} }=
	-\frac{i e \text{MW} \text{RXi}(W) \cos (\alpha -\beta )}{2 s_W}
	,
\end{autobreak}
\end{align}
\begin{align}
\begin{autobreak}
g_{H c_{W^{+}} \bar{c}_{W^{+}} }=
	-\frac{i e \text{MW} \text{RXi}(W) \cos (\alpha -\beta )}{2 s_W}
	,
\end{autobreak}
\end{align}
\begin{align}
\begin{autobreak}
g_{H c_{Z} \bar{c}_{Z} }=
	-\frac{i e \text{MZ} \text{RXi}(Z) \cos (\alpha -\beta )}{2 c_W s_W}
	,
\end{autobreak}
\end{align}
\begin{align}
\begin{autobreak}
g_{h c_{W^{-}} \bar{c}_{W^{-}} }=
	\frac{i e \text{MW} \text{RXi}(W) \sin (\alpha -\beta )}{2 s_W}
	,
\end{autobreak}
\end{align}
\begin{align}
\begin{autobreak}
g_{h c_{W^{+}} \bar{c}_{W^{+}} }=
	\frac{i e \text{MW} \text{RXi}(W) \sin (\alpha -\beta )}{2 s_W}
	,
\end{autobreak}
\end{align}
\begin{align}
\begin{autobreak}
g_{h c_{Z} \bar{c}_{Z} }=
	\frac{i e \text{MZ} \text{RXi}(Z) \sin (\alpha -\beta )}{2 c_W s_W}
	,
\end{autobreak}
\end{align}
\begin{align}
\begin{autobreak}
g_{H^{-} c_{\gamma} \bar{c}_{W^{-}} }=
	0
	,
\end{autobreak}
\end{align}
\begin{align}
\begin{autobreak}
g_{H^{-} c_{W^{+}} \bar{c}_{Z} }=
	0
	,
\end{autobreak}
\end{align}
\begin{align}
\begin{autobreak}
g_{H^{-} c_{Z} \bar{c}_{W^{-}} }=
	0
	,
\end{autobreak}
\end{align}
\begin{align}
\begin{autobreak}
g_{H^{+} c_{\gamma} \bar{c}_{W^{+}} }=
	0
	,
\end{autobreak}
\end{align}
\begin{align}
\begin{autobreak}
g_{H^{+} c_{W^{-}} \bar{c}_{Z} }=
	0
	,
\end{autobreak}
\end{align}
\begin{align}
\begin{autobreak}
g_{H^{+} c_{Z} \bar{c}_{W^{+}} }=
	0
	
\end{autobreak}
\end{align}
