\begin{align}
\begin{autobreak}
g_{G^{0} G^{-} W^{+} }=
	-\frac{e}{2 s_W}
	,
\end{autobreak}
\end{align}
\begin{align}
\begin{autobreak}
g_{G^{0} G^{+} W^{-} }=
	-\frac{e}{2 s_W}
	,
\end{autobreak}
\end{align}
\begin{align}
\begin{autobreak}
g_{G^{0} H \gamma }=
	0
	,
\end{autobreak}
\end{align}
\begin{align}
\begin{autobreak}
g_{G^{0} H Z }=
	\frac{e \cos (\alpha -\beta )}{2 c_W s_W}
	,
\end{autobreak}
\end{align}
\begin{align}
\begin{autobreak}
g_{G^{0} h \gamma }=
	0
	,
\end{autobreak}
\end{align}
\begin{align}
\begin{autobreak}
g_{G^{0} h Z }=
	-\frac{e \sin (\alpha -\beta )}{2 c_W s_W}
	,
\end{autobreak}
\end{align}
\begin{align}
\begin{autobreak}
g_{G^{0} H^{-} W^{+} }=
	0
	,
\end{autobreak}
\end{align}
\begin{align}
\begin{autobreak}
g_{G^{0} H^{+} W^{-} }=
	0
	,
\end{autobreak}
\end{align}
\begin{align}
\begin{autobreak}
g_{G^{-} G^{+} \gamma }=
	i e
	,
\end{autobreak}
\end{align}
\begin{align}
\begin{autobreak}
g_{G^{-} G^{+} Z }=
	-\frac{i e}{2 c_W s_W}
	+\frac{i e s_W}{c_W},
\end{autobreak}
\end{align}
\begin{align}
\begin{autobreak}
g_{G^{-} A W^{+} }=
	0
	,
\end{autobreak}
\end{align}
\begin{align}
\begin{autobreak}
g_{G^{-} H W^{+} }=
	-\frac{i e \cos (\alpha -\beta )}{2 s_W}
	,
\end{autobreak}
\end{align}
\begin{align}
\begin{autobreak}
g_{G^{-} h W^{+} }=
	\frac{i e \sin (\alpha -\beta )}{2 s_W}
	,
\end{autobreak}
\end{align}
\begin{align}
\begin{autobreak}
g_{G^{-} H^{+} \gamma }=
	0
	,
\end{autobreak}
\end{align}
\begin{align}
\begin{autobreak}
g_{G^{-} H^{+} Z }=
	0
	,
\end{autobreak}
\end{align}
\begin{align}
\begin{autobreak}
g_{G^{+} A W^{-} }=
	0
	,
\end{autobreak}
\end{align}
\begin{align}
\begin{autobreak}
g_{G^{+} H W^{-} }=
	\frac{i e \cos (\alpha -\beta )}{2 s_W}
	,
\end{autobreak}
\end{align}
\begin{align}
\begin{autobreak}
g_{G^{+} h W^{-} }=
	-\frac{i e \sin (\alpha -\beta )}{2 s_W}
	,
\end{autobreak}
\end{align}
\begin{align}
\begin{autobreak}
g_{G^{+} H^{-} \gamma }=
	0
	,
\end{autobreak}
\end{align}
\begin{align}
\begin{autobreak}
g_{G^{+} H^{-} Z }=
	0
	,
\end{autobreak}
\end{align}
\begin{align}
\begin{autobreak}
g_{A H \gamma }=
	0
	,
\end{autobreak}
\end{align}
\begin{align}
\begin{autobreak}
g_{A H Z }=
	\frac{e \sin (\alpha -\beta )}{2 c_W s_W}
	,
\end{autobreak}
\end{align}
\begin{align}
\begin{autobreak}
g_{A h \gamma }=
	0
	,
\end{autobreak}
\end{align}
\begin{align}
\begin{autobreak}
g_{A h Z }=
	\frac{e \cos (\alpha -\beta )}{2 c_W s_W}
	,
\end{autobreak}
\end{align}
\begin{align}
\begin{autobreak}
g_{A H^{-} W^{+} }=
	-\frac{e}{2 s_W}
	,
\end{autobreak}
\end{align}
\begin{align}
\begin{autobreak}
g_{A H^{+} W^{-} }=
	-\frac{e}{2 s_W}
	,
\end{autobreak}
\end{align}
\begin{align}
\begin{autobreak}
g_{H H^{-} W^{+} }=
	\frac{i e \sin (\alpha -\beta )}{2 s_W}
	,
\end{autobreak}
\end{align}
\begin{align}
\begin{autobreak}
g_{H H^{+} W^{-} }=
	-\frac{i e \sin (\alpha -\beta )}{2 s_W}
	,
\end{autobreak}
\end{align}
\begin{align}
\begin{autobreak}
g_{h H^{-} W^{+} }=
	\frac{i e \cos (\alpha -\beta )}{2 s_W}
	,
\end{autobreak}
\end{align}
\begin{align}
\begin{autobreak}
g_{h H^{+} W^{-} }=
	-\frac{i e \cos (\alpha -\beta )}{2 s_W}
	,
\end{autobreak}
\end{align}
\begin{align}
\begin{autobreak}
g_{H^{-} H^{+} \gamma }=
	i e
	,
\end{autobreak}
\end{align}
\begin{align}
\begin{autobreak}
g_{H^{-} H^{+} Z }=
	-\frac{i e}{2 c_W s_W}
	+\frac{i e s_W}{c_W}
\end{autobreak}
\end{align}
