\begin{align}
\begin{autobreak}
g_{G^{-} \gamma W^{+} }=
	-\frac{i e^2 v \bar{g}^{\rho \sigma }}{2 s_W}
	,
\end{autobreak}
\end{align}
\begin{align}
\begin{autobreak}
g_{G^{-} W^{+} Z }=
	-\frac{i e^2 v \bar{g}^{\rho \sigma }}{2 c_W}
	,
\end{autobreak}
\end{align}
\begin{align}
\begin{autobreak}
g_{G^{+} \gamma W^{-} }=
	-\frac{i e^2 v \bar{g}^{\rho \sigma }}{2 s_W}
	,
\end{autobreak}
\end{align}
\begin{align}
\begin{autobreak}
g_{G^{+} W^{-} Z }=
	-\frac{i e^2 v \bar{g}^{\rho \sigma }}{2 c_W}
	,
\end{autobreak}
\end{align}
\begin{align}
\begin{autobreak}
g_{H \gamma Z }=
	0
	,
\end{autobreak}
\end{align}
\begin{align}
\begin{autobreak}
g_{H W^{-} W^{+} }=
	\frac{i e^2 v \cos (\alpha -\beta ) \bar{g}^{\rho \sigma }}{2 s_W^2}
	,
\end{autobreak}
\end{align}
\begin{align}
\begin{autobreak}
g_{H Z Z }=
	\frac{i e^2 v \cos (\alpha -\beta ) \bar{g}^{\rho \sigma }}{2 c_W^2 s_W^2}
	,
\end{autobreak}
\end{align}
\begin{align}
\begin{autobreak}
g_{h \gamma Z }=
	0
	,
\end{autobreak}
\end{align}
\begin{align}
\begin{autobreak}
g_{h W^{-} W^{+} }=
	-\frac{i e^2 v \sin (\alpha -\beta ) \bar{g}^{\rho \sigma }}{2 s_W^2}
	,
\end{autobreak}
\end{align}
\begin{align}
\begin{autobreak}
g_{h Z Z }=
	-\frac{i e^2 v \sin (\alpha -\beta ) \bar{g}^{\rho \sigma }}{2 c_W^2 s_W^2}
	,
\end{autobreak}
\end{align}
\begin{align}
\begin{autobreak}
g_{H^{-} \gamma W^{+} }=
	0
	,
\end{autobreak}
\end{align}
\begin{align}
\begin{autobreak}
g_{H^{-} W^{+} Z }=
	0
	,
\end{autobreak}
\end{align}
\begin{align}
\begin{autobreak}
g_{H^{+} \gamma W^{-} }=
	0
	,
\end{autobreak}
\end{align}
\begin{align}
\begin{autobreak}
g_{H^{+} W^{-} Z }=
	0
	
\end{autobreak}
\end{align}
