\begin{align}
\begin{autobreak}
g_{G^{0} G^{0} \gamma Z }=
	0
	,
\end{autobreak}
\end{align}
\begin{align}
\begin{autobreak}
g_{G^{0} G^{0} W^{-} W^{+} }=
	\frac{i e^2 \bar{g}^{\rho \sigma }}{2 s_W^2}
	,
\end{autobreak}
\end{align}
\begin{align}
\begin{autobreak}
g_{G^{0} G^{0} Z Z }=
	\frac{i e^2 \bar{g}^{\rho \sigma }}{2 c_W^2 s_W^2}
	,
\end{autobreak}
\end{align}
\begin{align}
\begin{autobreak}
g_{G^{0} G^{-} \gamma W^{+} }=
	\frac{e^2 \bar{g}^{\rho \sigma }}{2 s_W}
	,
\end{autobreak}
\end{align}
\begin{align}
\begin{autobreak}
g_{G^{0} G^{-} W^{+} Z }=
	\frac{e^2 \bar{g}^{\rho \sigma }}{2 c_W}
	,
\end{autobreak}
\end{align}
\begin{align}
\begin{autobreak}
g_{G^{0} G^{+} \gamma W^{-} }=
	-\frac{e^2 \bar{g}^{\rho \sigma }}{2 s_W}
	,
\end{autobreak}
\end{align}
\begin{align}
\begin{autobreak}
g_{G^{0} G^{+} W^{-} Z }=
	-\frac{e^2 \bar{g}^{\rho \sigma }}{2 c_W}
	,
\end{autobreak}
\end{align}
\begin{align}
\begin{autobreak}
g_{G^{0} A W^{-} W^{+} }=
	0
	,
\end{autobreak}
\end{align}
\begin{align}
\begin{autobreak}
g_{G^{0} A Z Z }=
	0
	,
\end{autobreak}
\end{align}
\begin{align}
\begin{autobreak}
g_{G^{0} H^{-} \gamma W^{+} }=
	0
	,
\end{autobreak}
\end{align}
\begin{align}
\begin{autobreak}
g_{G^{0} H^{-} W^{+} Z }=
	0
	,
\end{autobreak}
\end{align}
\begin{align}
\begin{autobreak}
g_{G^{0} H^{+} \gamma W^{-} }=
	0
	,
\end{autobreak}
\end{align}
\begin{align}
\begin{autobreak}
g_{G^{0} H^{+} W^{-} Z }=
	0
	,
\end{autobreak}
\end{align}
\begin{align}
\begin{autobreak}
g_{G^{-} G^{+} \gamma \gamma }=
	2 i e^2 \bar{g}^{\rho \sigma }
	,
\end{autobreak}
\end{align}
\begin{align}
\begin{autobreak}
g_{G^{-} G^{+} \gamma Z }=
	-\frac{i e^2 \bar{g}^{\rho \sigma }}{c_W s_W}
	+\frac{2 i e^2 s_W \bar{g}^{\rho \sigma }}{c_W},
\end{autobreak}
\end{align}
\begin{align}
\begin{autobreak}
g_{G^{-} G^{+} W^{-} W^{+} }=
	\frac{i e^2 \bar{g}^{\rho \sigma }}{2 s_W^2}
	,
\end{autobreak}
\end{align}
\begin{align}
\begin{autobreak}
g_{G^{-} G^{+} Z Z }=
	-\frac{2 i e^2 \bar{g}^{\rho \sigma }}{c_W^2}
	+\frac{i e^2 \bar{g}^{\rho \sigma }}{2 c_W^2 s_W^2}
	+\frac{2 i e^2 s_W^2 \bar{g}^{\rho \sigma }}{c_W^2},
\end{autobreak}
\end{align}
\begin{align}
\begin{autobreak}
g_{G^{-} A \gamma W^{+} }=
	0
	,
\end{autobreak}
\end{align}
\begin{align}
\begin{autobreak}
g_{G^{-} A W^{+} Z }=
	0
	,
\end{autobreak}
\end{align}
\begin{align}
\begin{autobreak}
g_{G^{-} H \gamma W^{+} }=
	-\frac{i e^2 \cos (\alpha -\beta ) \bar{g}^{\rho \sigma }}{2 s_W}
	,
\end{autobreak}
\end{align}
\begin{align}
\begin{autobreak}
g_{G^{-} H W^{+} Z }=
	-\frac{i e^2 \cos (\alpha -\beta ) \bar{g}^{\rho \sigma }}{2 c_W}
	,
\end{autobreak}
\end{align}
\begin{align}
\begin{autobreak}
g_{G^{-} h \gamma W^{+} }=
	\frac{i e^2 \sin (\alpha -\beta ) \bar{g}^{\rho \sigma }}{2 s_W}
	,
\end{autobreak}
\end{align}
\begin{align}
\begin{autobreak}
g_{G^{-} h W^{+} Z }=
	\frac{i e^2 \sin (\alpha -\beta ) \bar{g}^{\rho \sigma }}{2 c_W}
	,
\end{autobreak}
\end{align}
\begin{align}
\begin{autobreak}
g_{G^{-} H^{+} \gamma \gamma }=
	0
	,
\end{autobreak}
\end{align}
\begin{align}
\begin{autobreak}
g_{G^{-} H^{+} \gamma Z }=
	0
	,
\end{autobreak}
\end{align}
\begin{align}
\begin{autobreak}
g_{G^{-} H^{+} W^{-} W^{+} }=
	0
	,
\end{autobreak}
\end{align}
\begin{align}
\begin{autobreak}
g_{G^{-} H^{+} Z Z }=
	0
	,
\end{autobreak}
\end{align}
\begin{align}
\begin{autobreak}
g_{G^{+} A \gamma W^{-} }=
	0
	,
\end{autobreak}
\end{align}
\begin{align}
\begin{autobreak}
g_{G^{+} A W^{-} Z }=
	0
	,
\end{autobreak}
\end{align}
\begin{align}
\begin{autobreak}
g_{G^{+} H \gamma W^{-} }=
	-\frac{i e^2 \cos (\alpha -\beta ) \bar{g}^{\rho \sigma }}{2 s_W}
	,
\end{autobreak}
\end{align}
\begin{align}
\begin{autobreak}
g_{G^{+} H W^{-} Z }=
	-\frac{i e^2 \cos (\alpha -\beta ) \bar{g}^{\rho \sigma }}{2 c_W}
	,
\end{autobreak}
\end{align}
\begin{align}
\begin{autobreak}
g_{G^{+} h \gamma W^{-} }=
	\frac{i e^2 \sin (\alpha -\beta ) \bar{g}^{\rho \sigma }}{2 s_W}
	,
\end{autobreak}
\end{align}
\begin{align}
\begin{autobreak}
g_{G^{+} h W^{-} Z }=
	\frac{i e^2 \sin (\alpha -\beta ) \bar{g}^{\rho \sigma }}{2 c_W}
	,
\end{autobreak}
\end{align}
\begin{align}
\begin{autobreak}
g_{G^{+} H^{-} \gamma \gamma }=
	0
	,
\end{autobreak}
\end{align}
\begin{align}
\begin{autobreak}
g_{G^{+} H^{-} \gamma Z }=
	0
	,
\end{autobreak}
\end{align}
\begin{align}
\begin{autobreak}
g_{G^{+} H^{-} W^{-} W^{+} }=
	0
	,
\end{autobreak}
\end{align}
\begin{align}
\begin{autobreak}
g_{G^{+} H^{-} Z Z }=
	0
	,
\end{autobreak}
\end{align}
\begin{align}
\begin{autobreak}
g_{A A \gamma Z }=
	0
	,
\end{autobreak}
\end{align}
\begin{align}
\begin{autobreak}
g_{A A W^{-} W^{+} }=
	\frac{i e^2 \bar{g}^{\rho \sigma }}{2 s_W^2}
	,
\end{autobreak}
\end{align}
\begin{align}
\begin{autobreak}
g_{A A Z Z }=
	\frac{i e^2 \bar{g}^{\rho \sigma }}{2 c_W^2 s_W^2}
	,
\end{autobreak}
\end{align}
\begin{align}
\begin{autobreak}
g_{A H^{-} \gamma W^{+} }=
	\frac{e^2 \bar{g}^{\rho \sigma }}{2 s_W}
	,
\end{autobreak}
\end{align}
\begin{align}
\begin{autobreak}
g_{A H^{-} W^{+} Z }=
	\frac{e^2 \bar{g}^{\rho \sigma }}{2 c_W}
	,
\end{autobreak}
\end{align}
\begin{align}
\begin{autobreak}
g_{A H^{+} \gamma W^{-} }=
	-\frac{e^2 \bar{g}^{\rho \sigma }}{2 s_W}
	,
\end{autobreak}
\end{align}
\begin{align}
\begin{autobreak}
g_{A H^{+} W^{-} Z }=
	-\frac{e^2 \bar{g}^{\rho \sigma }}{2 c_W}
	,
\end{autobreak}
\end{align}
\begin{align}
\begin{autobreak}
g_{H H \gamma Z }=
	0
	,
\end{autobreak}
\end{align}
\begin{align}
\begin{autobreak}
g_{H H W^{-} W^{+} }=
	\frac{i e^2 \bar{g}^{\rho \sigma }}{2 s_W^2}
	,
\end{autobreak}
\end{align}
\begin{align}
\begin{autobreak}
g_{H H Z Z }=
	\frac{i e^2 \bar{g}^{\rho \sigma }}{2 c_W^2 s_W^2}
	,
\end{autobreak}
\end{align}
\begin{align}
\begin{autobreak}
g_{H h W^{-} W^{+} }=
	0
	,
\end{autobreak}
\end{align}
\begin{align}
\begin{autobreak}
g_{H h Z Z }=
	0
	,
\end{autobreak}
\end{align}
\begin{align}
\begin{autobreak}
g_{H H^{-} \gamma W^{+} }=
	-\frac{i e^2 \sin (\alpha -\beta ) \bar{g}^{\rho \sigma }}{2 s_W}
	,
\end{autobreak}
\end{align}
\begin{align}
\begin{autobreak}
g_{H H^{-} W^{+} Z }=
	-\frac{i e^2 \sin (\alpha -\beta ) \bar{g}^{\rho \sigma }}{2 c_W}
	,
\end{autobreak}
\end{align}
\begin{align}
\begin{autobreak}
g_{H H^{+} \gamma W^{-} }=
	-\frac{i e^2 \sin (\alpha -\beta ) \bar{g}^{\rho \sigma }}{2 s_W}
	,
\end{autobreak}
\end{align}
\begin{align}
\begin{autobreak}
g_{H H^{+} W^{-} Z }=
	-\frac{i e^2 \sin (\alpha -\beta ) \bar{g}^{\rho \sigma }}{2 c_W}
	,
\end{autobreak}
\end{align}
\begin{align}
\begin{autobreak}
g_{h h \gamma Z }=
	0
	,
\end{autobreak}
\end{align}
\begin{align}
\begin{autobreak}
g_{h h W^{-} W^{+} }=
	\frac{i e^2 \bar{g}^{\rho \sigma }}{2 s_W^2}
	,
\end{autobreak}
\end{align}
\begin{align}
\begin{autobreak}
g_{h h Z Z }=
	\frac{i e^2 \bar{g}^{\rho \sigma }}{2 c_W^2 s_W^2}
	,
\end{autobreak}
\end{align}
\begin{align}
\begin{autobreak}
g_{h H^{-} \gamma W^{+} }=
	-\frac{i e^2 \cos (\alpha -\beta ) \bar{g}^{\rho \sigma }}{2 s_W}
	,
\end{autobreak}
\end{align}
\begin{align}
\begin{autobreak}
g_{h H^{-} W^{+} Z }=
	-\frac{i e^2 \cos (\alpha -\beta ) \bar{g}^{\rho \sigma }}{2 c_W}
	,
\end{autobreak}
\end{align}
\begin{align}
\begin{autobreak}
g_{h H^{+} \gamma W^{-} }=
	-\frac{i e^2 \cos (\alpha -\beta ) \bar{g}^{\rho \sigma }}{2 s_W}
	,
\end{autobreak}
\end{align}
\begin{align}
\begin{autobreak}
g_{h H^{+} W^{-} Z }=
	-\frac{i e^2 \cos (\alpha -\beta ) \bar{g}^{\rho \sigma }}{2 c_W}
	,
\end{autobreak}
\end{align}
\begin{align}
\begin{autobreak}
g_{H^{-} H^{+} \gamma \gamma }=
	2 i e^2 \bar{g}^{\rho \sigma }
	,
\end{autobreak}
\end{align}
\begin{align}
\begin{autobreak}
g_{H^{-} H^{+} \gamma Z }=
	-\frac{i e^2 \bar{g}^{\rho \sigma }}{c_W s_W}
	+\frac{2 i e^2 s_W \bar{g}^{\rho \sigma }}{c_W},
\end{autobreak}
\end{align}
\begin{align}
\begin{autobreak}
g_{H^{-} H^{+} W^{-} W^{+} }=
	\frac{i e^2 \bar{g}^{\rho \sigma }}{2 s_W^2}
	,
\end{autobreak}
\end{align}
\begin{align}
\begin{autobreak}
g_{H^{-} H^{+} Z Z }=
	-\frac{2 i e^2 \bar{g}^{\rho \sigma }}{c_W^2}
	+\frac{i e^2 \bar{g}^{\rho \sigma }}{2 c_W^2 s_W^2}
	+\frac{2 i e^2 s_W^2 \bar{g}^{\rho \sigma }}{c_W^2}
\end{autobreak}
\end{align}
